enqueue

pulse/examples/steel/LListWithTail.fst
@@ -256,7 +256,7 @@ let read_head
 
 (* END helpers to unfold definitions just to prove that I can read the head pointer of a list and check its value to determine whether the list is empty or not *)
 
-val pop
+val dequeue
   (#a: Type)
   (x: t a)
   (l: Ghost.erased (list (cell a)))
@@ -267,10 +267,10 @@ val pop
     (requires (fun _ -> Cons? l /\ next_hd == next (L.hd l)))
     (ensures (fun _ res _ -> Cons? l /\ snd res == Ghost.hide (L.tl l) /\ (fst res).tail == x.tail))
 
-let pop
+let dequeue
   #a x l next_hd
 =
-  let (l2: Ghost.erased (l: list (cell a) { Cons? l })) = Ghost.hide (Ghost.reveal l) in
+  let (l2: Ghost.erased (l: list (cell a) { Cons? l })) = Ghost.hide (Ghost.reveal l) in // necessary otherwise refinement type checking fails
   change_equiv_slprop
     (llist_fragment x.head l)
     (pts_to x.head full_perm (Some (L.hd l2)) `star` llist_fragment (next (L.hd l2)) (L.tl l2))
@@ -284,7 +284,7 @@ let pop
     (fun _ -> ());
   (x', Ghost.hide (L.tl l2))
 
-let test_read_head_pop
+let test_read_head_dequeue
   (#a: Type)
   (x: t a)
   (l: Ghost.erased (list (cell a)))
@@ -305,490 +305,42 @@ let test_read_head_pop
     (x, l)
   | Some c ->
     let n = next c in
-    let res = pop x l n in // explicit let-binding necessary, otherwise "effects SteelF and Steel cannot be composed"
+    let res = dequeue x l n in // explicit let-binding necessary, otherwise "effects SteelF and Steel cannot be composed"
     res
 
-
-(*
-  noop ();
-  change_equiv_slprop
-    (llist_with_tail x l)
-    (
-
-  change_equiv_slprop (
-    (pts_to x.head full_perm (Some (L.hd l)) `star` llist_fragment (next (L.hd l)) (L.tl l)) `star` pts_to (next_last x.head l) full_perm None) `star` pure (x.tail == Ghost.reveal (next_last x.head l))
-  ) (
-    pts_to x.head full_perm (Some (L.hd l)) `star` ((llist_fragment (next (L.hd l)) (L.tl l) `star` pts_to (next_last x.head l) full_perm None) `star` pure (x.tail == Ghost.reveal (next_last x.head l)))
-  ) ();
-(*  
-  change_equiv_slprop (
-    pts_to x.head full_perm (Some (L.hd l)) `star` ((llist_fragment (next (L.hd l)) (L.tl l) `star` pts_to (next_last x.head l) full_perm None) `star` pure (x.tail == Ghost.reveal (next_last x.head l)))
-  ) (llist_with_tail x l) ();
-*)
-  change_equiv_slprop (
-    pts_to x.head full_perm (Some (L.hd l)) `star` ((llist_fragment (next (L.hd l)) (L.tl l) `star` pts_to (next_last x.head l) full_perm None) `star` pure (x.tail == Ghost.reveal (next_last x.head l)))
-  ) (
-    (pts_to x.head full_perm (Some (L.hd l)) `star` llist_fragment (next (L.hd l)) (L.tl l)) `star` pts_to (next_last x.head l) full_perm None) `star` pure (x.tail == Ghost.reveal (next_last x.head l)
-  )  
-  ();
-  ()
-
-[@"opaque_to_smt"]
-let llist_with_tail_read_next_head_snoc
-  (#a: Type) (x: t a) (l: Ghost.erased (list (cell a)))
-: Ghost (option (cell a) & slprop)
-  (requires (Cons? l /\ Cons? (unsnoc_hd l)))
-  (ensures (fun (v, q) -> llist_with_tail x l `equiv` (pts_to (next (L.hd l)) full_perm v `star` q) /\ v == Some (L.hd (L.tl l))))
-= 
-  let hd = unsnoc_hd l in
-  let tl = unsnoc_tl l in
-  let r = (pts_to (next_last x.head hd) full_perm (Some (Ghost.reveal tl)) `star` pts_to (next tl) full_perm None `star` pts_to x.tail full_perm (next_last x.head hd)) in
-  let (v, q) = llist_fragment_read_head_cons (next (L.hd l)) (L.tl l) in
-  star_congruence (pts_to x.head full_perm (Some (L.hd l))) (llist_fragment
-  
-  star_congruence (llist_fragment x.head hd) r (pts_to x.head full_perm v `star` q) r;
-  assert (
-    ((pts_to x.head full_perm v `star` q) `star` r)
-    `equiv`
-    (pts_to x.head full_perm v `star` (q `star` r))
-  ) by (canon ());
-  (Ghost.reveal v, (q `star` r))
-
-
-
-(*
-  slassert (llist_with_tail x l);
-  change_equiv_slprop
-    (llist_with_tail x l)
-    (pts_to x.head full_perm (fst q) `star` snd q)
-    ();
-  let r = read #a #full_perm #(fst q) x.head in
-  change_equiv_slprop
-    (pts_to x.head full_perm (fst q) `star` snd q)
-    (llist_with_tail x l)
-    ();
-  (r, snd q)
-
-
-
-(*
-
-let llist_with_tail_read
+val enqueue
   (#a: Type)
   (x: t a)
   (l: Ghost.erased (list (cell a)))
-: Steel (option (cell a) & slprop)
-  (llist_with_tail x l)
-  (fun q -> llist_with_tail x l) // pts_to x.head full_perm (fst q) `star` snd q)
-  (requires (fun _ -> True))
-  (ensures (fun _ q _ ->
-    llist_with_tail x l `equiv` (pts_to x.head full_perm (fst q) `star` snd q) /\
-    Cons? l == Some? (fst q)
-  ))
-=
-  noop ();
-  let q : Ghost.erased (option (cell a)) & slprop = llist_with_tail_read_2 x l in
-  let q2 = snd q in
-  noop ()
-
-  slassert (llist_with_tail x l);
-  change_equiv_slprop
+  (v: a)
+: Steel (t a & Ghost.erased (list (cell a)))
     (llist_with_tail x l)
-    (pts_to x.head full_perm (fst q) `star` snd q)
-    ();
-  let r = read #a #full_perm #(fst q) x.head in
-  change_equiv_slprop
-    (pts_to x.head full_perm (fst q) `star` snd q)
-    (llist_with_tail x l)
-    ();
-  (r, snd q)
-
-
-
-
-
-let rec llist_with_tail_fragment (#a: Type0) (x: t a) (hd: Ghost.erased (cell a)) (tl: Ghost.erased (list (cell a))) : Tot slprop (decreases (Ghost.reveal tl)) =
-  pts_to x.head full_perm hd `star`
-  begin match Ghost.reveal tl with
-  | [] -> pure (x.tail == x.head)
-  | a' :: q -> llist_with_tail_fragment ({ head = next hd; tail = x.tail }) a' q
-  end
-
-let llist_with_tail_fragment_aux (#a: Type0) (x: t a) (hd: Ghost.erased (cell a)) (tl: Ghost.erased (list (cell a))) : Tot slprop =
-  match Ghost.reveal tl with
-  | [] -> pure (x.tail == x.head)
-  | a' :: q -> llist_with_tail_fragment ({ head = next hd; tail = x.tail }) a' q
-
-let llist_with_tail_fragment_unfold
-(#a: Type0) (x: t a) (hd: Ghost.erased (cell a)) (tl: Ghost.erased (list (cell a))) : Lemma
-  (llist_with_tail_fragment x hd tl ==
-  pts_to x.head full_perm hd `star` llist_with_tail_fragment_aux x hd tl
-)
-= ()
-
-let llist_with_tail_fragment_nil
-  (#a: Type0) (x: t a) (hd: Ghost.erased (cell a)) (tl: Ghost.erased (list (cell a)))
-: Lemma
-  (requires (Nil? tl))
-  (ensures (llist_with_tail_fragment x hd tl == (pts_to x.head full_perm hd `star` pure (x.tail == x.head))))
-=
-  ()
-
-let llist_with_tail_fragment_cons
-  (#a: Type0) (x: t a) (hd: Ghost.erased (cell a)) (tl: Ghost.erased (list (cell a)))
-: Lemma
-  (requires (Cons? tl))
-  (ensures (llist_with_tail_fragment x hd tl == (pts_to x.head full_perm hd `star` llist_with_tail_fragment ({ head = next hd; tail = x.tail }) (L.hd tl) (L.tl tl))))
-=
-  ()
-
-let llist_with_tail_fragment_rev_aux (#a: Type0) (x: t a) (hd: Ghost.erased (list (cell a))) (tl: Ghost.erased (cell a)) : Tot slprop =
-  match Ghost.reveal hd with
-  | [] -> pure (x.tail == x.head)
-  | a' :: q -> llist_with_tail_fragment_rev ({ head = next a'; tail = x.tail }) q tl
-
-let llist_with_tail_fragment_rev_unfold
-  (#a: Type0) (x: t a) (hd: Ghost.erased (list (cell a))) (tl: Ghost.erased (cell a))
-: Lemma
-  (llist_with_tail_fragment_rev x hd tl ==
-  pts_to x.tail full_perm tl `star` llist_with_tail_fragment_rev_aux x hd tl)
-= ()
-
-let llist_with_tail_fragment_rev_nil (#a: Type0) (x: t a) (hd: Ghost.erased (list (cell a))) (tl: Ghost.erased (cell a)) : Lemma
-  (requires (Nil? hd))
-  (ensures (llist_with_tail_fragment_rev x hd tl == (pts_to x.tail full_perm tl `star` pure (x.tail == x.head))))
-= ()
-
-let llist_with_tail_fragment_rev_cons (#a: Type0) (x: t a) (hd: Ghost.erased (list (cell a))) (tl: Ghost.erased (cell a)) : Lemma
-  (requires (Cons? hd))
-  (ensures (llist_with_tail_fragment_rev x hd tl == (pts_to x.tail full_perm tl `star` llist_with_tail_fragment_rev ({ head = next (L.hd hd); tail = x.tail }) (L.tl hd) tl)))
-= ()
-
-let llist_with_tail (#a: Type0) (x: t a) (l: Ghost.erased (list (cell a))) : Tot slprop =
-  match Ghost.reveal l with
-  | [] -> pure (is_null x.head == true) `star` pure (is_null x.tail == true)
-  | hd :: tl -> llist_with_tail_fragment x hd tl `star` pure (is_null (next (L.last l)) == true)
-
-let llist_with_tail_nil
-  (#a: Type)
-  (x: t a)
-  (l: Ghost.erased (list (cell a)))
-: Lemma
-  (requires (Nil? l))
-  (ensures (llist_with_tail x l == pure (is_null x.head == true) `star` pure (is_null x.tail == true)))
-= ()
-
-let llist_with_tail_cons
-  (#a: Type0) (x: t a) (l: Ghost.erased (list (cell a)))
-: Lemma
-  (requires (Cons? l))
-  (ensures (llist_with_tail x l == llist_with_tail_fragment x (L.hd l) (L.tl l) `star` pure (is_null (next (L.last l)) == true)))
-= ()
-
-let pure_star_interp (p:slprop u#a) (q:prop) (m:mem)
-   : Lemma (interp (p `star` pure q) m <==>
-            interp p m /\ q)
-=
-  pure_star_interp p q m;
-  emp_unit p
-
-let pure_cut
-  (p: slprop)
-  (q: prop)
-  (f: (m: mem) -> Lemma (requires (interp p m)) (ensures q))
-: Steel unit
-    p
-    (fun _ -> p)
+    (fun res -> llist_with_tail (fst res) (snd res))
     (requires (fun _ -> True))
-    (ensures (fun _ _ _ -> q))
+    (ensures (fun _ res _ -> datas (snd res) == datas l `L.append` [v] /\ (fst res).head == x.head))
+
+let enqueue
+  #a x l v
 =
-  change_slprop p (p `star` pure q) (fun m -> f m; pure_star_interp p q m);
-  let _ : squash q = elim_pure q in
-  noop ()
-
-val intro_llist_nil (a:Type)
-   : SteelT unit emp (fun _ -> llist_with_tail (null_llist #a) [])
-
-let intro_llist_nil a =
-  change_slprop emp (llist_with_tail (null_llist #a) [])
-    (fun m ->
-      pure_interp (is_null (null_llist #a).head == true) m;
-      pure_star_interp (pure (is_null (null_llist #a).head == true)) (is_null (null_llist #a).tail == true) m;
-      norm_spec [delta; zeta] ((llist_with_tail (null_llist #a) [])))
-
-val intro_llist_cons_nil'
-  (a: Type)
-  (ptr: t a)
-  (x: cell a)
-  (m: mem)
-: Lemma
-  (requires (
-    is_null (next x) == true /\ ptr.tail == ptr.head /\
-    interp (pts_to ptr.head full_perm x) m
-  ))
-  (ensures (interp (llist_with_tail ptr [x]) m))
-
-let intro_llist_cons_nil'
-  a ptr x m
-=
-  norm_spec [delta; zeta] (llist_with_tail ptr [x]);
-  pure_star_interp (llist_with_tail_fragment ptr x []) (is_null (next (L.last [x])) == true) m;
-  norm_spec [delta; zeta] (llist_with_tail_fragment ptr x []);
-  pure_star_interp (pts_to ptr.head full_perm x) (ptr.tail == ptr.head) m
-
-let intro_llist_cons_nil
-  (a: Type)
-  (ptr: t a)
-  (x: cell a)
-: Steel unit
-    (pts_to ptr.head full_perm x)
-    (fun _ -> llist_with_tail ptr [x])
-    (requires (fun _ -> is_null (next x) == true /\ ptr.tail == ptr.head))
-    (ensures (fun _ _ _ -> True))
-=
+  let n : cellptr a = alloc None in
+  let c = mk_cell n v in
+  elim_pure (x.tail == Ghost.reveal (next_last x.head l));
+  change_slprop (pts_to (next_last x.head l) full_perm None) (pts_to x.tail full_perm None) (fun _ -> ());
+  write #(option (cell a)) #None x.tail (Some c); // FIXME: WHY WHY WHY do I need to explicitly provide the implicits?
+  change_slprop (pts_to x.tail full_perm (Some c) `star` emp) (llist_fragment (next_last x.head l) [c]) (fun _ -> ());
+  let l2 : Ghost.erased (list (cell a)) = Ghost.hide (l `L.append` [c]) in
+  change_slprop (llist_fragment x.head l `star` llist_fragment (next_last x.head l) [c]) (llist_fragment x.head l2) (fun _ -> llist_fragment_append x.head l [c]);
+  let y = { head = x.head; tail = n } in
+  change_slprop (llist_fragment x.head l2) (llist_fragment y.head l2) (fun _ -> ());
+  L.lemma_append_last l [c];
+  next_last_correct y.head (l `L.append` [c]);
+  intro_pure (y.tail == Ghost.reveal (next_last y.head l2));
+  change_slprop (pts_to n full_perm None) (pts_to (next_last y.head l2) full_perm None) (fun _ -> ());
+  L.map_append data l [c]; // must appear before the last change_slprop
+  let res : t a & Ghost.erased (list (cell a)) = (y, l2) in
   change_slprop
-    (pts_to ptr.head full_perm x)
-    (llist_with_tail ptr [x])
-    (fun m -> intro_llist_cons_nil' a ptr x m)
-
-val push_nil
-  (a: Type)
-  (x: a)
-: Steel
-    (t a & Ghost.erased (list (cell a)))
-    (emp)
-    (fun z -> llist_with_tail (fst z) (snd z))
-    (requires (fun _ -> True))
-    (ensures (fun _ z _ -> datas (snd z) == [x]))
-
-#push-options "--ide_id_info_off"
-
-let push_nil
-  a e
-=
-  let x = mk_cell null e in
-  let px = alloc x in
-  let ptr = {head = px ; tail = px} in
-  change_slprop
-    (pts_to px full_perm x)
-    (pts_to ptr.head full_perm x)
+    (llist_fragment y.head l2 `star` pts_to (next_last y.head l2) full_perm None `star` pure (y.tail == Ghost.reveal (next_last y.head l2)))
+    (llist_with_tail (fst res) (snd res))
     (fun _ -> ());
-  intro_llist_cons_nil a ptr x;
-  let z = (ptr, Ghost.hide [x]) in
-  change_slprop
-    (llist_with_tail ptr [x])
-    (llist_with_tail (fst z) (snd z))
-    (fun _ -> ());
-  z
-
-let pts_to_not_null_intro
-  (#a:Type u#0)
-  (x:ref a)
-  (p:perm)
-  (v: Ghost.erased a)
-: Steel unit (pts_to x p v) (fun _ -> pts_to x p v)
-  (requires (fun _ -> True))
-  (ensures (fun _ _ _ -> is_null x == false))
-=
-  pure_cut (pts_to x p v) (is_null x == false) (fun m ->
-    pts_to_not_null x p v m
-  )
-
-let llist_is_nil_intro
-  (a: Type)
-  (ptr: t a)
-  (l: Ghost.erased (list (cell a)))
-  (m: mem)
-: Lemma
-  (requires (interp (llist_with_tail ptr l) m))
-  (ensures (Nil? l == is_null ptr.head))
-=
-  match Ghost.reveal l with
-  | [] ->
-    llist_with_tail_nil ptr l;
-    pure_star_interp (pure (is_null ptr.head == true)) (is_null ptr.tail == true) m;
-    pure_interp (is_null ptr.head == true) m
-  | hd :: tl ->
-    llist_with_tail_cons ptr l;
-    pure_star_interp (llist_with_tail_fragment ptr (L.hd l) (L.tl l)) (is_null (next (L.last l)) == true) m;
-    llist_with_tail_fragment_unfold ptr hd tl;
-    elim_star (pts_to ptr.head full_perm hd) (llist_with_tail_fragment_aux ptr hd tl) m;
-    pts_to_not_null ptr.head full_perm hd m
-
-val llist_is_nil
-  (a: Type)
-  (ptr: t a)
-  (l: Ghost.erased (list (cell a)))
-: Steel
-    bool
-    (llist_with_tail ptr l)
-    (fun _ -> llist_with_tail ptr l)
-    (requires (fun _ -> True))
-    (ensures (fun _ b _ -> Nil? l == b))
-
-let llist_is_nil
-  a ptr l
-=
-  let res = (is_null ptr.head) in
-  pure_cut (llist_with_tail ptr l) (Nil? l == res) (fun m ->
-    llist_is_nil_intro a ptr l m
-  );
+  // it seems that nothing must come before the last change_slprop and the return value
   res
-
-val intro_llist_cons_cons'
-  (a: Type)
-  (ptr: t a)
-  (ptr0 : t a)
-  (x: cell a)
-  (q: Ghost.erased (list (cell a)))
-  (m: mem)
-: Lemma
-  (requires (interp
-    (llist_with_tail ptr0 q `star` pts_to ptr.head full_perm x)
-    m /\
-    ptr0.head == next x /\ ptr0.tail == ptr.tail /\ Cons? q == true
-  ))
-  (ensures (interp
-    (llist_with_tail ptr (x :: q))
-  ) m)
-
-let intro_llist_cons_cons'
-  a ptr ptr0 x q m
-=
-  (* destruct the hypothesis *)
-  llist_with_tail_cons ptr0 q;
-  assert ((
-    (llist_with_tail_fragment ptr0 (L.hd q) (L.tl q) `star` pure (is_null (next (L.last q)) == true)) `star` pts_to ptr.head full_perm x
-    ) `equiv` (
-    (pts_to ptr.head full_perm x `star` llist_with_tail_fragment ptr0 (L.hd q) (L.tl q)) `star` pure (is_null (next (L.last q)) == true)
-  )) by (Steel.Memory.Tactics.canon ());
-  pure_star_interp
-    (pts_to ptr.head full_perm x `star` llist_with_tail_fragment ptr0 (L.hd q) (L.tl q))
-    (is_null (next (L.last q)) == true)
-    m;
-  (* construct the conclusion *)
-  assert (ptr0 == ({ head = next x; tail = ptr.tail }));
-  assert (L.last (x :: q) == L.last q);
-  llist_with_tail_fragment_cons ptr x q;
-  pure_star_interp
-    (llist_with_tail_fragment ptr x q)
-    (is_null (next (L.last (x :: q))) == true)
-    m;
-  llist_with_tail_cons ptr (x :: q)
-
-let intro_llist_cons_cons
-  (a: Type)
-  (ptr: t a)
-  (ptr0 : t a)
-  (x: cell a)
-  (q: Ghost.erased (list (cell a)))
-: Steel
-    unit
-    (llist_with_tail ptr0 q `star` pts_to ptr.head full_perm x)
-    (fun _ -> llist_with_tail ptr (x :: q))
-    (requires (fun _ -> ptr0.head == next x /\ ptr0.tail == ptr.tail /\ Cons? q == true))
-    (ensures (fun _ _ _ -> True))
-=
-  change_slprop
-    (llist_with_tail ptr0 q `star` pts_to ptr.head full_perm x)
-    (llist_with_tail ptr (x :: q))
-    (fun m -> intro_llist_cons_cons' a ptr ptr0 x q m)
-
-val push_cons
-  (a: Type)
-  (ptr: t a)
-  (x: a)
-  (q: Ghost.erased (list (cell a)))
-: Steel
-    (t a & Ghost.erased (list (cell a)))
-    (llist_with_tail ptr q)
-    (fun z -> llist_with_tail (fst z) (snd z))
-    (requires (fun _ -> Cons? q == true))
-    (ensures (fun _ z _ -> datas (snd z) == x :: datas q))
-
-let push_cons
-  a ptr0 e q
-=
-  let x = mk_cell ptr0.head e in
-  let px = alloc x in
-  let ptr = {head = px ; tail = ptr0.tail} in
-  change_slprop
-    (pts_to px full_perm x)
-    (pts_to ptr.head full_perm x)
-    (fun _ -> ());
-  intro_llist_cons_cons a ptr ptr0 x q;
-  let z = (ptr, Ghost.hide (x :: q)) in
-  change_slprop
-    (llist_with_tail ptr (Ghost.hide (x :: q)))
-    (llist_with_tail (fst z) (snd z))
-    (fun _ -> ());
-  z
-
-val push
-  (a: Type)
-  (ptr: t a)
-  (x: a)
-  (q: Ghost.erased (list (cell a)))
-: Steel
-    (t a & Ghost.erased (list (cell a)))
-    (llist_with_tail ptr q)
-    (fun z -> llist_with_tail (fst z) (snd z))
-    (requires (fun _ -> True))
-    (ensures (fun _ z _ -> datas (snd z) == x :: datas q))
-
-let push
-  a ptr x q
-=
-  let is_nil = llist_is_nil a ptr q in
-  if is_nil
-  then begin
-    drop (llist_with_tail ptr q);
-    push_nil a x
-  end
-  else begin
-    noop (); // FIXME: WHY WHY WHY? (Alternatively, let res = push_cons ... in res will also work, but still, WHY?)
-    push_cons a ptr x q
-  end
-
-val intro_llist_cons_snoc'
-  (a: Type)
-  (ptr: t a)
-  (ptr0 : t a)
-  (x: cell a)
-  (q: Ghost.erased (list (cell a)))
-  (m: mem)
-: Lemma
-  (requires (
-    Cons? q == true /\
-    interp
-      (llist_with_tail ptr0 q `star` pts_to (next (L.last q)) full_perm x)
-    m /\
-    ptr0.head == ptr.head /\ ptr.tail == next (L.last q)
-  ))
-  (ensures (interp
-    (llist_with_tail ptr (q `L.append` [x]))
-  ) m)
-
-let intro_llist_cons_snoc'
-  a ptr ptr0 x q m
-=
-  (* destruct the hypothesis *)
-  llist_with_tail_cons ptr0 q;
-  assert ((
-    (llist_with_tail_fragment ptr0 (L.hd q) (L.tl q) `star` pure (is_null (next (L.last q)) == true)) `star` pts_to ptr.head full_perm x
-    ) `equiv` (
-    (pts_to ptr.head full_perm x `star` llist_with_tail_fragment ptr0 (L.hd q) (L.tl q)) `star` pure (is_null (next (L.last q)) == true)
-  )) by (Steel.Memory.Tactics.canon ());
-  pure_star_interp
-    (pts_to ptr.head full_perm x `star` llist_with_tail_fragment ptr0 (L.hd q) (L.tl q))
-    (is_null (next (L.last q)) == true)
-    m;
-  (* construct the conclusion *)
-  assert (ptr0 == ({ head = next x; tail = ptr.tail }));
-  assert (L.last (x :: q) == L.last q);
-  llist_with_tail_fragment_cons ptr x q;
-  pure_star_interp
-    (llist_with_tail_fragment ptr x q)
-    (is_null (next (L.last (x :: q))) == true)
-    m;
-  llist_with_tail_cons ptr (x :: q)
